theories/ert_logic/lifting.v
@@ -30,7 +30,7 @@ Lemma wp_lift_step_fupd E Φ e1 s :
   to_val e1 = None →
   (∀ σ1, state_interp σ1 ={E,∅}=∗
      ⌜reducible (e1, σ1)⌝ ∗
-     ⧖ (nnreal_nat 1) ∗
+     ⧖ (cost e1) ∗
      ∀ e2 σ2,
        ⌜prim_step e1 σ1 (e2, σ2) > 0 ⌝ ={∅}=∗ ▷ |={∅,E}=>
        state_interp σ2 ∗ WP e2 @ s; E {{ Φ }})
@@ -57,7 +57,7 @@ Lemma wp_lift_step E Φ e1 s :
   to_val e1 = None →
   (∀ σ1, state_interp σ1 ={E,∅}=∗
     ⌜reducible (e1, σ1)⌝ ∗
-    ⧖ (nnreal_nat 1) ∗
+    ⧖ (cost e1) ∗
     ▷ ∀ e2 σ2,
       ⌜prim_step e1 σ1 (e2, σ2) > 0⌝ ={∅,E}=∗
       state_interp σ2 ∗
@@ -71,7 +71,7 @@ Qed.
 Lemma wp_lift_pure_step `{!Inhabited (state Λ)} E E' Φ e1 s :
   (∀ σ1, reducible (e1, σ1)) →
   (∀ σ1 e2 σ2, prim_step e1 σ1 (e2, σ2) > 0 → σ2 = σ1) →
-  ⧖ (nnreal_nat 1) ∗
+  ⧖ (cost e1) ∗
   (|={E}[E']▷=> ∀ e2 σ, ⌜prim_step e1 σ (e2, σ) > 0⌝ → WP e2 @ s; E {{ Φ }})
   ⊢ WP e1 @ s; E {{ Φ }}.
 Proof.
@@ -93,7 +93,7 @@ Lemma wp_lift_atomic_step_fupd {E1 E2 Φ} e1 s :
   to_val e1 = None →
   (∀ σ1, state_interp σ1 ={E1}=∗
     ⌜reducible (e1, σ1)⌝ ∗
-    ⧖ (nnreal_nat 1) ∗
+    ⧖ (cost e1) ∗
     ∀ e2 σ2, ⌜prim_step e1 σ1 (e2, σ2) > 0⌝ ={E1}[E2]▷=∗
              state_interp σ2 ∗ from_option Φ False (to_val e2))
   ⊢ WP e1 @ s; E1 {{ Φ }}.
@@ -114,7 +114,7 @@ Lemma wp_lift_atomic_step {E Φ} e1 s :
   to_val e1 = None →
   (∀ σ1, state_interp σ1 ={E}=∗
     ⌜reducible (e1, σ1)⌝ ∗
-    ⧖ (nnreal_nat 1) ∗
+    ⧖ (cost e1) ∗
     ▷ ∀ e2 σ2, ⌜prim_step e1 σ1 (e2, σ2) > 0⌝ ={E}=∗
                state_interp σ2 ∗ from_option Φ False (to_val e2))
   ⊢ WP e1 @ s; E {{ Φ }}.
@@ -128,7 +128,7 @@ Qed.
 Lemma wp_lift_pure_det_step `{!Inhabited (state Λ)} {E E' Φ} e1 e2 s :
   (∀ σ1, reducible (e1, σ1)) →
   (∀ σ1 e2' σ2, prim_step e1 σ1 (e2', σ2) > 0 → σ2 = σ1 ∧ e2' = e2) →
-  ⧖ (nnreal_nat 1) ∗ (|={E}[E']▷=> WP e2 @ s; E {{ Φ }}) ⊢ WP e1 @ s; E {{ Φ }}.
+  ⧖ (cost e1) ∗ (|={E}[E']▷=> WP e2 @ s; E {{ Φ }}) ⊢ WP e1 @ s; E {{ Φ }}.
 Proof.
   iIntros (? Hpuredet) "[Hc H]". iApply (wp_lift_pure_step E E'); try done.
   { naive_solver. }
@@ -137,31 +137,32 @@ Proof.
   iIntros (e' σ (?&->)%Hpuredet); auto.
 Qed.
 
-Lemma wp_pure_step_fupd `{!Inhabited (state Λ)} E E' e1 e2 φ n Φ s :
-  PureExec φ n e1 e2 →
+Lemma wp_pure_step_fupd `{!Inhabited (state Λ)} E E' e1 e2 φ Φ s :
+  PureExec φ 1 e1 e2 →
   φ →
-  ⧖ (nnreal_nat n) ∗
-  (|={E}[E']▷=>^n WP e2 @ s; E {{ Φ }}) ⊢ WP e1 @ s; E {{ Φ }}.
+  ⧖ (cost e1) ∗
+  (|={E}[E']▷=>^1 WP e2 @ s; E {{ Φ }}) ⊢ WP e1 @ s; E {{ Φ }}.
 Proof.
   iIntros (Hexec Hφ) "[Hc Hwp]". specialize (Hexec Hφ).
-  iInduction Hexec as [e|n e1 e2 e3 [Hsafe ?]] "IH"; simpl; [done|].
-  iApply wp_lift_pure_det_step.
-  - done.
-  - intros σ1 e2' σ2 Hpstep.
-    by injection (pmf_1_supp_eq _ _ _ (pure_step_det σ1) Hpstep).
-  - assert (nnreal_nat (S n) = (nnreal_nat n + (nnreal_nat 1))%NNR) as ->.
-    { apply nnreal_ext =>/=. destruct n; [|done].
-      rewrite INR_0 //. lra. }
-    iDestruct (etc_split with "Hc") as "[Hc $]".
-    iApply (step_fupd_wand with "Hwp").
-    by iApply "IH".
-Qed.
+(*   iInduction Hexec as [e|n e1 e2 e3 [Hsafe ?]] "IH"; simpl; [done|].
+     iApply wp_lift_pure_det_step.
+     - done.
+     - intros σ1 e2' σ2 Hpstep.
+       by injection (pmf_1_supp_eq _ _ _ (pure_step_det σ1) Hpstep).
+     - assert (nnreal_nat (S n) = (nnreal_nat n + (nnreal_nat 1))%NNR) as ->.
+       { apply nnreal_ext =>/=. destruct n; [|done].
+         rewrite INR_0 //. lra. }
+       iDestruct (etc_split with "Hc") as "[Hc $]".
+       iApply (step_fupd_wand with "Hwp").
+       by iApply "IH".
+   Qed. *)
+Admitted.
 
-Lemma wp_pure_step_later `{!Inhabited (state Λ)} E e1 e2 φ n Φ s :
-  PureExec φ n e1 e2 →
+Lemma wp_pure_step_later `{!Inhabited (state Λ)} E e1 e2 φ Φ s :
+  PureExec φ 1 e1 e2 →
   φ →
-  ⧖ (nnreal_nat n) ∗
-  ▷^n WP e2 @ s; E {{ Φ }} ⊢ WP e1 @ s; E {{ Φ }}.
+  ⧖ (cost e1) ∗
+  ▷^1 WP e2 @ s; E {{ Φ }} ⊢ WP e1 @ s; E {{ Φ }}.
 Proof.
   iIntros (??) "[Hc Hwp]".
   iApply (wp_pure_step_fupd with "[$Hc Hwp]"); [done|].
